\documentclass[a4paper,12pt, twoside]{article}
\usepackage[russian]{babel}

\begin{document}
Упражнение 1: \\
Выполнить бета-редукцию $\lambda$-терма $((\lambda a.(\lambda b.b\;b)\;(\lambda b.b\;b))\;b)\;((\lambda c.(c\;b))\;(\lambda a.a)).$ \\

$((\lambda a.(\lambda b.b\;b)\;(\lambda b.b\;b))\;b)\;((\lambda c.(c\;b))\;(\lambda a.a))=((\lambda b.b\;b)\;(\lambda b.b\;b))\;((\lambda c.(c\;b))\;(\lambda a.a))=(\Omega)\;((\lambda c.(c\;b))\;(\lambda a.a))=(\Omega)\;((\lambda a.a)\;b)=(\Omega)\;(b)=\Omega\;b$ \newline

Упражнение 2: \\
Доказать, что $S\;K\;K = I.$ \\
Доказательство: \\

$S\;K\;K = (\lambda x\;y\;z.x\;z\;(y\;z))\;(\lambda x\;y.x)\;(\lambda x\;y.x)=(\lambda x\;y.(\lambda u\;v.u)\;y\;(x\;y))\;(\lambda x\;y.x)=(\lambda x.(\lambda u\;v.u)\;x\;((\lambda p\;q.p)\;x))=\lambda x.(\lambda u\;v.u)\;x\;\lambda q.x=\lambda x.x=I$
\end{document}